Added proof rule for refining fairness assumptions

src/temporal_logic/lemmas.lean
@@ -345,6 +345,9 @@ begin [temporal]
 end
 (eventually_weaken _)
 
+instance inf_often_postponable (p : cpred) : postponable (◻◇p) :=
+by constructor ; simp [eventually_inf_often]
+
 lemma coincidence {p q : cpred} {Γ}
     (Hp : Γ ⊢ ◇◻p)
     (Hq : Γ ⊢ ◻◇q)
@@ -404,18 +407,6 @@ lemma eventually_and {Γ p q : cpred}
 begin [temporal]
   eventually h₁ ⊢,
   split ; assumption
-end
-
-lemma eventually_exists (P : α → cpred)
-: ◇(∃∃ x, P x) = ∃∃ x, ◇P x :=
-begin
-  funext1,
-  unfold eventually p_exists,
-  split
-  ; intro H
-  ; cases H with i H
-  ; cases H with j H
-  ; exact ⟨_,_,H⟩ ,
 end
 
 /- Actions -/
@@ -500,6 +491,18 @@ begin [temporal]
     apply True_p_and },
 end
 
+protected theorem leads_to_disj_gen {t}
+  {p q : t → cpred}
+  {Γ : cpred}
+  (P₀ : Γ ⊢ ∀∀ i, p i ~> q i)
+: Γ ⊢ (∃∃ i, p i) ~> (∃∃ i, q i) :=
+begin [temporal]
+  apply temporal.leads_to_disj _,
+  intro j,
+  apply temporal.leads_to_strengthen_rhs _ _ (P₀ j),
+  apply p_exists_intro
+end
+
 section induction
 
 variables {α' : Type u}
@@ -514,8 +517,7 @@ begin [temporal]
   have h₂ : ∀∀ V : β, p ⋀ (f ≃ V) ~> q,
   { intro V,
     wf_induction V,
-    apply temporal.leads_to_strengthen_rhs _ _,
-    show q ⋁ q ⟹ q,
+    apply temporal.leads_to_strengthen_rhs (q ⋁ q),
     { simp [or_self], },
     apply temporal.leads_to_cancellation (P _),
     rw_using : (p ⋀ (f ≺≺ x)) = (∃∃v, ↑(v << x) ⋀ (p ⋀ (f ≃ v))),
@@ -690,207 +692,5 @@ begin
 end
 
 end
-
-section simulation
-
-section pair
-
-variables {α' : Type u} {β' : Type u₀} {γ' : Type u₁}
-variables (x : tvar α') (y : tvar β') (z : tvar γ')
-
-def pair : tvar (α' × β') :=
-lifted₂ prod.mk x y
-
-notation `⦃` x `,` l:(foldl `,` (h t, pair h t) x `⦄`)  := l
-
-@[simp]
-lemma pair_model (i : ℕ) :
-i ⊨ ⦃x,y⦄ = (i ⊨ y,i ⊨ x) :=
-by { cases x, cases y, refl }
-
-@[reducible]
-def pair.fst : var (α' × β') α' :=
-↑(@prod.fst α' β')
-
-@[simp]
-def pair.fst_mk (x : tvar α') (y : tvar β')
-: pair.fst ;; ⦃y,x⦄ = x :=
-by lifted_pred
-
--- @[simp]
-def pair.fst_mk' (x : tvar α') (y : tvar β')
-: ↑(@prod.fst α' β') ;; ⦃y,x⦄ = x :=
-pair.fst_mk _ _
-
-end pair
-
-parameters {α' : Type u} {β' : Type u₀} {γ' : Type u₁ }
-parameters {p : pred' (α'×γ')} {q : pred' (β'×γ')}
-parameters {A : act (α'×γ')} {C : act (β'×γ')}
-parameters {J : pred' (α'×β'×γ')}
-
-variables (x : tvar α') (y : tvar β') (z : tvar γ')
-
-def SPEC₀ (v : tvar α') (o : tvar γ') : cpred :=
-p ;; ⦃ o,v ⦄ ⋀
-◻⟦ ⦃o,v⦄ <> A ⟧
-
-def SPEC₁ (v : tvar β') (o : tvar γ') : cpred :=
-q ;; ⦃ o,v ⦄ ⋀
-◻⟦ ⦃o,v⦄ <> C ⟧
-
-parameter [inhabited α']
-parameter SIM₀ : ∀ v o, (v,o) ⊨ q → ∃ w, (w,o) ⊨ p ∧ (w,v,o) ⊨ J
-parameter SIM
-: ∀ {w v o} v' o',
-  (w,v,o) ⊨ J →
-  C (v,o) (v',o') →
-  ∃ w', A (w,o) (w',o') ∧
-        (w',v',o') ⊨ J
-
-parameters (v : tvar β') (o : tvar γ')
-
-parameters {Γ : cpred}
-parameters H : Γ ⊢ SPEC₁ v o
-
-section witness
-variables (i : ℕ) (Hi : i ⊨ Γ)
-include H Hi
-
-open classical
-
-private noncomputable def ww : Π j : ℕ, { w : α' // j ≥ i → (w,j ⊨ v,j ⊨ o) ⊨ J }
- | j :=
-if h : j > i then
-     have h₀ : j ≥ 1,
-       by { apply succ_le_of_lt,
-            apply nat.lt_of_le_of_lt (nat.zero_le i) h },
-     have h₁ : i ≤ j - 1,
-       by { rw ← add_le_to_le_sub _ ; assumption },
-     have Hdec : j - 1 < j,
-       by { apply nat.sub_lt_of_pos_le, apply zero_lt_one,
-            assumption },
-     let hw := (ww (j-1)).property h₁ in
-     have Hstep : C (j - 1 ⊨ v, j - 1 ⊨ o) (j ⊨ v, j ⊨ o),
-       begin
-         clear_except H Hi h₀ h₁ h, replace H := (H.apply _ Hi).right ((j-1) - i),
-         simp at H, rw [← nat.add_sub_assoc,nat.add_sub_cancel_left,← succ_sub] at H
-         ; apply H <|> assumption,
-       end,
-     let x := some (SIM (j ⊨ v) (j ⊨ o) hw Hstep) in
-     have h₁ : j ≥ i → (x, j ⊨ v, j ⊨ o) ⊨ J,
-       from assume _, (some_spec (SIM (j ⊨ v) (j ⊨ o) hw Hstep)).right,
-     ⟨x,h₁⟩
-else if h' : i ≤ j then
-     have h : i = j,
-       by { apply le_antisymm h', apply le_of_not_gt, assumption },
-     have h₀ : (j ⊨ v, j ⊨ o) ⊨ q,
-          begin
-            clear_except H Hi h,
-            have := H.left.apply _ Hi, simp at this,
-            subst i, apply this,
-          end,
-     let x₀ := some (SIM₀ (j ⊨ v) (j ⊨ o) h₀) in
-     have h₁ : j ≥ i → (x₀, j ⊨ v, j ⊨ o) ⊨ J,
-       from assume _, (some_spec (SIM₀ (j ⊨ v) (j ⊨ o) h₀)).right,
-     ⟨x₀,h₁⟩
-else
-  have h₁ : j ≥ i → (default α', j ⊨ v, j ⊨ o) ⊨ J,
-    by { intro, exfalso, apply h', assumption, },
-  ⟨default α',h₁⟩
-
-private noncomputable def ww' (j : ℕ) := (ww i Hi j).val
-
-end witness
-include H SIM₀ SIM
-
-lemma simulation
-: Γ ⊢ ∃∃ w, SPEC₀ w o :=
-begin
-  simp [SPEC₀],
-  lifted_pred keep,
-  let w := ww' SIM₀ @SIM v o H _ a,
-  existsi (⟨ w ⟩ : tvar α'),
-  split,
-  intro i,
-  { simp,
-    generalize h : w (x + i) = z,
-    have h' : succ (x + i) > x,
-    { apply lt_succ_of_le, apply nat.le_add_right },
-    simp [w], rw [ww',ww], simp [dif_pos h'],
-    rw ← h,
-    apply_some_spec, simp, intros, assumption, },
-  { dsimp [w,ww'], rw ww, simp,
-    apply_some_spec,
-    simp, intros, assumption, },
-end
-omit H
-lemma simulation'
-: (∃∃ c, SPEC₁ c o) ⟹ (∃∃ a, SPEC₀ a o) :=
-begin [temporal]
-  rw p_exists_p_imp,
-  intros x h,
-  apply simulation SIM₀ @SIM _ _ h,
-end
-
-end simulation
-
-section witness_construction
-
-parameters {α' : Sort u}
-parameters {p J : pred' α'}
-parameters {A : act α'}
-
-parameters H₀ : p ⟹ J
-parameters FIS₀ : ∃ σ, σ ⊨ p
-parameters FIS : ∀ σ, σ ⊨ J → ∃ σ', A σ σ'
-parameters INV : ∀ σ σ', σ ⊨ J → A σ σ' → σ' ⊨ J
-
-open classical
-
-include H₀ INV
-
-def A' : plift α' × unit → plift α' × unit → Prop :=
-A on (plift.down ∘ prod.fst)
-
-parameters [_inst : inhabited α']
-
-include FIS₀ FIS _inst
-lemma witness_construction
-: ⊩ ∃∃ v, p ;; v ⋀ ◻⟦ v <> A ⟧ :=
-begin
-  intro,
-  let o : tvar unit := ↑(),
-  let C : unit × unit → unit × unit → Prop := λ _ _, true,
-  let prj : var (plift α' × unit) α' := ↑(@plift.down α') ;; pair.fst,
-  let p' : pred' (plift α' × unit) := p ;; prj,
-  have _inst : inhabited (plift α') := ⟨ plift.up (default α') ⟩,
-  let J' : pred' (plift α' × unit × unit) := J ;; ↑(@plift.down α') ;; pair.fst,
-  have := @simulation _ _ _ p' (@True $ unit × unit) (A' H₀ INV) C J' _ _ _ o o Γ _,
-  begin [temporal]
-    revert this,
-    let f : tvar (plift α') → tvar α' := λ v, ↑(λ x : plift α', x.down) ;; v,
-    let SPEC := @SPEC₀ _ _ p' (A' H₀ INV),
-    let SPEC' := λ (v : tvar α'), p ;; v ⋀ ◻⟦ v <> A ⟧,
-    apply p_exists_imp_p_exists' (λ w, SPEC w o) SPEC' f,
-    intro, simp only [SPEC,f,SPEC',SPEC₀,p',prj,proj_assoc,pair.fst_mk,A'],
-    monotonicity, rw [action_on,coe_over_comp,proj_assoc,pair.fst_mk'],
-    refl,
-  end,
-  { intros,
-    revert FIS₀,
-    apply exists_imp_exists' plift.up,
-    introv h, split, simp [p',h],
-    simp [J'], apply ew_str H₀ _ h, },
-  { introv hJ hC, simp [J'] at hJ,
-    have := FIS (w.down) hJ, revert this,
-    apply exists_imp_exists' plift.up,
-    introv hA, simp [A'], split,
-    { apply INV _ _ hJ hA  },
-    { apply hA } },
-  { simp [SPEC₁,C], }
-end
-
-end witness_construction
 
 end temporal
