src/temporal_logic/persistent.lean
@@ -24,6 +24,10 @@ instance and_persistent {p q : cpred} [persistent p] [persistent q]
 : persistent (p ⋀ q) :=
 by { constructor, simp [henceforth_and,is_persistent], }
 
+instance coe_persistent (p : Prop)
+: persistent (p : cpred) :=
+by { constructor, cases classical.prop_complete p ; subst p ; simp, }
+
 instance true_persistent
 : persistent (True : cpred) :=
 by { constructor, simp, }
@@ -35,6 +39,21 @@ by { constructor, simp, }
 instance forall_persistent {p : α → cpred} [∀ i, persistent (p i)]
 : persistent (p_forall p) :=
 by { constructor, simp [henceforth_forall,is_persistent], }
+
+instance not_exists_persistent {p : α → cpred} [∀ i, persistent (- p i)]
+: persistent (- p_exists p) :=
+by { constructor, simp [p_not_p_exists,henceforth_forall,is_persistent], }
+
+instance exists_persistent {p : α → cpred} [∀ i, persistent (p i)]
+: persistent (p_exists p) :=
+by { constructor, apply mutual_entails,
+     apply henceforth_str,
+     apply p_exists_elim, intro, rw ← is_persistent (p x),
+     monotonicity, apply p_exists_intro, }
+
+instance not_forall_persistent {p : α → cpred} [∀ i, persistent (- p i)]
+: persistent (- p_forall p) :=
+by { constructor, simp [p_not_p_forall], apply is_persistent }
 
 def list_persistent (xs : list cpred) :=
 Π q ∈ xs, persistent q
@@ -84,6 +103,38 @@ begin
       apply henceforth_str, } }
 end
 
+class postponable (p : cpred) : Prop :=
+  (postpone : ◇p = p)
+export postponable (postpone)
+
+lemma p_imp_postpone (Γ p q : cpred) [postponable q]
+  (h : tl_imp Γ p q)
+: tl_imp Γ (◇p) q :=
+begin
+  rw ← postpone q,
+  monotonicity h,
+end
+
+instance (p : cpred) : postponable (◇p) :=
+by { constructor, simp [eventually_eventually] }
+
+instance forall_postponable (p : α → cpred) [∀ i, postponable (p i)]
+: postponable (p_forall p) :=
+⟨ begin
+    apply mutual_entails,
+    { rw [p_entails_of_fun],
+      introv h, rw p_forall_to_fun, intro i,
+      rw ← postpone (p i), revert h, apply p_impl_revert,
+      revert Γ, change (_ ⟹ _),
+      monotonicity, rw [p_entails_of_fun],
+      introv h, apply p_forall_revert h },
+    apply eventually_weaken
+  end ⟩
+
+instance exists_postponable (p : α → cpred) [∀ i, postponable (p i)]
+: postponable (p_exists p) :=
+by constructor ; simp [eventually_exists,postpone]
+
 lemma persistent_to_henceforth {p q : cpred}
   (h : ◻ p ⊢ q)
 : ◻ p ⊢ ◻ q :=
@@ -95,5 +146,7 @@ instance has_coe_to_fun_henceforth (Γ p q : cpred) : has_coe_to_fun (Γ ⊢ ◻
 
 instance has_coe_to_fun_leads_to (Γ p q : cpred) : has_coe_to_fun (Γ ⊢ p ~> q) :=
 temporal.has_coe_to_fun_henceforth _ _ _
+
+
 
 end temporal
