src/temporal_logic/fairness.lean
@@ -1,0 +1,108 @@
+-- import temporal_logic.tactic
+import temporal_logic.lemmas
+
+universes u
+
+open predicate temporal
+
+namespace temporal
+namespace fairness
+
+section defs
+
+variables p q A : cpred
+
+def wf : cpred :=
+◇◻p ⟶ ◻◇A
+
+def sf : cpred :=
+◻◇p ⟶ ◻◇A
+
+def sched : cpred :=
+◇◻p ⟶ ◻◇q ⟶ ◻◇A
+
+instance persistent_sched : persistent (sched p q A) :=
+by { unfold sched, apply_instance }
+
+end defs
+
+section one_to_one
+
+variables Γ p q A : cpred
+variables p' q' A' : cpred
+
+variables H₀ : Γ ⊢ p' ⋀ q' ~> p
+variables H₁ : Γ ⊢ ◻◇p ⟶ ◇◻p ⋁ ◻◇-p'
+variables H₂ : Γ ⊢ ◻(A ⟶ A')
+variables H₃ : Γ ⊢ p' ⋀ q' ~> q
+include H₀ H₁ H₂ H₃
+
+lemma replacement
+: Γ ⊢ sched p q A ⟶ sched p' q' A' :=
+begin [temporal]
+  simp [sched], intros,
+  have swc := coincidence a_1 a_2,
+  have wc : ◇◻p,
+  { assume_negation, simp at h,
+    rw [p_or_comm,← p_not_p_imp] at H₁, simp at H₁,
+    apply H₁ _ a_1,
+    apply inf_often_of_leads_to H₀ swc, },
+  have sc : ◻◇q,
+  { apply inf_often_of_leads_to H₃ swc, },
+  replace a := a wc sc, revert a,
+  { persistent, monotonicity, apply H₂, },
+end
+
+end one_to_one
+section splitting
+
+variables {t : Sort u}
+variables w p q A : t → cpred
+variables Γ p' q' A' : cpred
+
+-- TODO(Simon) Weaken proof obligation `H₀`. We can do with ◻◇_ ⟶ ◻◇ _
+-- instead of _ ~> _
+
+-- variables H₀ : Γ ⊢ ∀∀ i, ◻◇(p' ⋀ q' ⋀ w i) ⟶ ◻◇p i ⋀ q i ⋀ w i
+variables H₀ : Γ ⊢ ∀∀ i, p' ⋀ q' ⋀ w i ~> p i ⋀ q i ⋀ w i
+variables H₁ : Γ ⊢ ∀∀ i, ◇(p i ⋀ w i) ⟶ ◇◻p' ⟶ ◇◻(p i ⋀ w i)
+variables H₂ : Γ ⊢ ∀∀ i, ◻(A i ⟶ A')
+variables H₃ : Γ ⊢ ◻(p' ⋀ q' ⟶ ∃∃ i, w i)
+include H₀ H₁ H₂ H₃
+
+open temporal
+lemma splitting
+: Γ ⊢ (∀∀ i, sched (p i) (q i) (A i)) ⟶ sched p' q' A' :=
+begin [temporal]
+  intro H₅,
+  simp [sched] at *, intros hp' hq',
+  have H₇ := inf_often_of_leads_to (temporal.leads_to_disj_gen  H₀) _,
+  replace H₇ : ∃∃ (i : t), ◇(p i ⋀ q i ⋀ w i),
+  { henceforth at H₇, rw eventually_exists at H₇, },
+  { cases H₇ with i H₇,
+    have H₉ := H₁ i _ hp',
+    have : ◻◇q i,
+    { have := inf_often_of_leads_to (H₀ i) _, revert this,
+      { monotonicity only, lifted_pred },
+      rw_using : (p' ⋀ q' ⋀ w i) = (p' ⋀ w i ⋀ q'),
+      { lifted_pred },
+      apply coincidence _ hq',
+      { apply stable_and_of_stable_of_stable hp',
+        revert H₉, monotonicity only p_and_elim_right _ _ _, }, },
+    have := H₅ i _ this,
+    { revert this, monotonicity only,
+      apply H₂ i },
+    { revert H₉, monotonicity only, lifted_pred, },
+    { revert H₇, monotonicity only, lifted_pred }, },
+  { have := coincidence hp' hq', revert this,
+    monotonicity only,
+    simp, intros hp hq,
+    have := H₃ hp hq,
+    revert this, apply p_exists_p_imp_p_exists,
+    intros i hw, repeat { split <|> assumption }, } ,
+end
+
+end splitting
+
+end fairness
+end temporal
